KripkeGameAnalysis/GenericExtras/Array.lean
@@ -1,0 +1,72 @@
+import Mathlib.Data.Finset.Basic
+
+namespace Finset
+end Finset
+
+namespace Array
+
+def setAtIndexPreservingLength (value : Fin n → α) (arr : { a : Array α // a.size = n }) (i : Fin n) : { a : Array α // a.size = n } :=
+  ⟨arr.val.set i (value i), by simp only [size_set]; exact arr.property⟩
+
+instance : RightCommutative (setAtIndexPreservingLength val) := {
+  right_comm := by
+    intro arr a1 a2
+    simp only [Subtype.mk.injEq, setAtIndexPreservingLength]
+    by_cases h : a1 = a2
+    · rw [h]
+    · rw [Array.set_comm (val a1) (val a2) arr (by revert h; contrapose!; exact Fin.eq_of_val_eq)]
+}
+
+lemma setAtIndexPreservingLength_eq {value : Fin n → α}
+                                    {arr : { a : Array α // a.size = n }} {i j: Fin n} :
+    (setAtIndexPreservingLength value arr i).val[j]'(by simp [(setAtIndexPreservingLength value arr i).property]) = if i = j then value i else arr.val[j] := by
+  simp only [setAtIndexPreservingLength]
+  by_cases h : i = j
+  · simp [h]
+  · simp only [Fin.getElem_fin, h, ↓reduceIte]
+    rw [Array.getElem_set_ne _ _ _ _ _ _]
+    simp [Fin.val_ne_of_ne h]
+
+def setAtIndices (a : Array α) (a_size : a.size = n) (indices : Finset (Fin n)) (value : Fin n → α) : Array α :=
+  (indices.val.foldl (setAtIndexPreservingLength value) ⟨a, a_size⟩).val
+
+theorem setAtIndices_size : (setAtIndices a a_size indices value).size = a.size := by
+  dsimp only [setAtIndices]
+  set res := indices.val.foldl (setAtIndexPreservingLength value) ⟨a, a_size⟩
+  rw [res.property, a_size]
+
+theorem setAtIndices_eq (a : Array α) (a_size : a.size = n) :
+    (setAtIndices a a_size indices value)[i]'(by simp [setAtIndices_size, a_size]) = if i ∈ indices then value i else a[i] := by
+  dsimp only [setAtIndices]
+  revert a
+  induction indices using Finset.induction_on with
+  | empty => simp
+  | insert headIndex_not_in_indices ih => next nextIndex restIndices =>
+      intro a a_size
+      simp only [Finset.insert_val_of_not_mem headIndex_not_in_indices]
+      simp only [Multiset.foldl_cons, Finset.mem_insert]
+      rw [ih _ _]
+      by_cases h : i ∈ restIndices
+      · simp [h]
+      · simp only [h, ↓reduceIte, or_false]
+        rw [setAtIndexPreservingLength_eq (value := value) (arr := ⟨a, a_size⟩) (i := nextIndex) (j := i)]
+        by_cases h' : i = nextIndex
+        · simp [h']
+        · simp [h']; tauto
+
+def setValueAtIndices {α : Type} (a : Array α) (a_size : a.size = n)
+                         (indices : Finset (Fin n)) (value : α) : Array α :=
+  setAtIndices a a_size indices (fun _ => value)
+
+theorem setValueAtIndices_size {α : Type} (a : Array α) (a_size : a.size = n)
+                                (indices : Finset (Fin n)) (value : α) :
+    (setValueAtIndices a a_size indices value).size = a.size :=
+  by simp only [setValueAtIndices]; exact setAtIndices_size
+
+theorem setValueAtIndices_eq {α : Type} (a : Array α) (a_size : a.size = n)
+                                (indices : Finset (Fin n)) (value : α) (i : Fin n) :
+    (setValueAtIndices a a_size indices value)[i]'(by simp [setValueAtIndices_size, a_size]) =
+    if i ∈ indices then value else a[i] :=
+  by simp only [setValueAtIndices]; rw [setAtIndices_eq]
+
+end Array
